---
title: "Formation of Partial Differential Equations (Part-2)"
author: "Siju Swamy"
date: "2024-07-25"
categories: [session note]
image: chem1.png
---
## Formation of PDE by Elimination of Arbitrary Function

To form a partial differential equation (PDE) by eliminating an arbitrary function from a given equation, follow these steps:

>*Example 1:* Find the PDE of the equation $z = f(x, y)$. where $f(x, y)$ is an arbitrary function of $x$ and $y$.

**SOlution:**

Step 1: Differentiate with Respect to $x$ and $y$

Differentiate the given equation with respect to $x$ and $y$ to form new equations involving the partial derivatives.

Differentiate with respect to $x$:

$$
\frac{\partial z}{\partial x} = \frac{\partial f(x, y)}{\partial x}
$$

Let $p = \frac{\partial z}{\partial x}$:

$$
p = f_x(x, y)
$$

Differentiate with respect to $y$:

$$
\frac{\partial z}{\partial y} = \frac{\partial f(x, y)}{\partial y}
$$

Let $q = \frac{\partial z}{\partial y}$:

$$
q = f_y(x, y)
$$

Step 2: Form the PDE

Divide the equations for $p$ and $q$:

$$
\frac{p}{q} = \frac{f_x(x, y)}{f_y(x, y)}
$$

Since $f(x, y)$ is arbitrary, $f_x(x, y)$ and $f_y(x, y)$ are just partial derivatives of the function. The relationship simplifies to:

$$
\frac{p}{q} = 1
$$

So, the PDE is:

$$
p = q
$$

>*Example 2:* Form a PDE from the general dependancy relationship, $z=yf\left(\frac{y}{x}\right)$ by eliminating the arbitrary function.

**Solution:**

Given static equation is $$z=yf\left(\frac{y}{x}\right)$$ {#eq-eqn-1}

Differentiating (@eq-eqn-1) partially with respect to $x$, we get:

$$\dfrac{\partial z}{\partial x}=yf'\left(\frac{y}{x}\right)\left(-\dfrac{y}{x^2}\right)$$  

or $$f'\left(\frac{y}{x}\right)=-\frac{x^2}{y^2}p$$ {#eq-eqn-2}

Differentiating (@eq-eqn-1) partially with respect to $x$, we get:

$$\dfrac{\partial z}{\partial y}=yf'\left(\frac{y}{x}\right)\left(\dfrac{1}{x}\right)+f\left(\frac{y}{x}\right)$$ {#eq-eqn-3}

Using (@eq-eqn-1), and (@eq-eqn-2) in (@eq-eqn-3), we get:

\begin{align*}
q&=\dfrac{y}{x}\times \left(\dfrac{x^2}{y^2}\right)p+\dfrac{z}{y}\\
&=-\frac{x}{y}p+\frac{z}{y}\\
\implies z&=px+qy
\end{align*}

>*Example 2:* Form a PDE from the equation $z=f(x^2-y^2)$, where $f$ is an arbitrary function.

**Solution:**

Given $$z=f(x^2-y^2)$$ {#eq-eqnp2}

Differentiating (@eq-eqnp2) partially with respect to $x$ and $y$, we get:

\begin{align}
p&=f'(x^2-y^2)\times 2x \\ 
q&=f'(x^2-y^2)\times -2y 
\end{align}

 $$\therefore \dfrac{p}{q}=-\frac{x}{y}\implies py+qx=0$$



